src/Provers.v
@@ -1,5 +1,6 @@
 Require Import List.
 Require Import Expr.
+Require Import EquivDec.
 
 (** TODO: This is going to be interesting...
 Section Unify.
@@ -32,14 +33,14 @@ Section Prover.
 
 Definition assumptionProver : ProverT fs.
   red.
-  refine (fix assumptionProver hyps (goal : expr fs nil nil None) : hlist (fun e => @exprD _ fs _ _ HNil HNil None e) hyps -> option (exprD HNil HNil goal) :=
+  refine (fix assumptionProver hyps (goal : expr fs nil nil tvProp) : hlist (fun e => @exprD _ fs _ _ HNil HNil tvProp e) hyps -> option (exprD HNil HNil goal) :=
     match hyps with
       | nil => fun _ => None
       | exp :: b => fun pfHyps => 
 (*        match vs as vs return forall exp : expr fs vs None, hlist (@qexprD _ fs) (existT (fun vs => expr fs vs None) vs exp :: b) -> _ with
           | nil => fun exp pfHyps => 
           *)
-        if exprEq goal exp then Some _ else assumptionProver b goal (hlist_tl pfHyps)
+        if seq_dec goal exp then Some _ else assumptionProver b goal (hlist_tl pfHyps)
 (*          | _ => fun _ pfHyps => assumptionProver b goal (hlist_tl pfHyps)
         end exp
 *)
@@ -63,16 +64,16 @@ Section BabyOmega.
 
   Definition types' := {| Impl := nat; Eq := fun x y => match eq_nat_dec x y with left Heq => Some Heq | _ => None end |} :: types.
   Definition fs' : functions types' :=
-    {| Domain := Some FO :: Some FO :: nil;
-      Range := None; Denotation := eq |}
-    :: {| Domain := (Some FO :: Some FO :: nil) : list (tvar types');
-      Range := Some FO; Denotation := plus |}
+    {| Domain := tvTrans FO :: tvTrans FO :: nil;
+      Range := tvProp; Denotation := eq |}
+    :: {| Domain := (tvTrans FO :: tvTrans FO :: nil) : list (tvar types');
+      Range := tvTrans FO; Denotation := plus |}
     :: fs (_ :: nil).
 
   Definition DMatch' f args :=
     option (match Range (get fs' f) as T return (expr fs' nil nil T -> Type) with
-              | Some f0 => fun _ : expr fs' nil nil (Some f0) => Empty_set
-              | None => fun goal : expr fs' nil nil None => exprD HNil HNil goal
+              | tvTrans f0 => fun _ : expr fs' nil nil (tvTrans f0) => Empty_set
+              | tvProp => fun goal : expr fs' nil nil tvProp  => exprD HNil HNil goal
             end (Func f args)).
 
   Definition DMatch (f : fin fs') : Type :=
@@ -82,13 +83,13 @@ Section BabyOmega.
     red.
     refine (fun _ goal _ =>
       match goal in expr _ _ _ T return option (match T return expr _ _ _ T -> Type with
-                                                | None => fun goal => exprD HNil HNil goal
+                                                | tvProp => fun goal => exprD HNil HNil goal
                                                 | _ => fun _ => Empty_set
                                               end goal) with
         | Func f args =>
           finIfz f DMatch
             (fun args => hlistDestruct args (DMatch' _) 
-              (fun x y => if exprEq x y then Some _ else None))
+              (fun x y => if seq_dec x y then Some _ else None))
             (fun _ _ => None) args
         | _ => None
       end);
