src/SepExprTests.v
@@ -1,0 +1,146 @@
+Require Import Heaps.
+Require Import SepExpr.
+Require Import EquivDec.
+Require Import List.
+
+Set Implicit Arguments.
+
+Module SepExpr (B : Heap).
+  Module ST := SepTheoryX.SepTheoryX B.  
+  Module Sep := SepExpr.SepExpr B.
+
+  (** Just a test separation logic predicate **)
+  Section Tests.
+    Variable f : forall a b, nat -> ST.hprop a b nil.
+    Variable h : forall a b, nat -> ST.hprop a b nil.
+    Variable i : forall a b, nat -> ST.hprop a b nil.
+    Variable g : bool -> nat -> nat -> nat.
+
+    Ltac isConst e :=
+      match e with
+        | true => true
+        | false => true
+        | O => true
+        | S ?e => isConst e
+        | _ => false
+      end.
+
+    Definition nat_type : type :=
+      {| Impl := nat 
+       ; Eq := fun x y => match equiv_dec x y with
+                            | left pf => Some pf
+                            | _ => None 
+                          end
+       |}.
+
+
+    Fixpoint all a b (f : nat -> ST.hprop a b nil) (n : nat) : ST.hprop a b nil :=
+      match n with
+        | 0 => f 0
+        | S n => ST.star (f (S n)) (all f n)
+      end.
+
+    Fixpoint allb a b (f : nat -> ST.hprop a b nil) (n m : nat) : ST.hprop a b nil :=
+      match n with
+        | 0 => f m
+        | S n => ST.star (f (m - S n)) (allb f n m)
+      end.
+
+
+    Goal forall a b c, @ST.himp a b c (ST.star (allb (@h a b) 15 15) (allb (@f a b) 15 15)) (ST.star (all (@f a b) 15) (all (@h a b) 15)).
+      simpl all. simpl allb.
+      intros. Sep.reflect isConst (@nil type). 
+      simple eapply ApplyCancelSep.
+      lazy.
+      reflexivity.
+(*
+      Transparent himp.
+      unfold himp. simpl.
+      Set Printing All.
+      
+       cbv beta iota zeta delta [CancelSep hash_left sepCancel].
+
+      
+
+(*      Time compute.
+      Eval compute in (functionTypeD (map (@tvarD types) nil) (@tvarD types (Some (FS (FS FO))))).
+
+      About Build_signature.
+*)
+      pose (types := (defaultType b :: defaultType a :: nat_type :: nil)).
+      change (himp (types := types) (pcType := Some (FS FO)) (stateType := Some FO)
+        (funcs := (Build_signature (types := types) nil (Some (FS (FS FO))) x :: (@nil (signature types))))
+        (sfuncs := Build_ssignature (types := types) (Some (FS FO)) (Some FO) (Some (FS (FS FO)) :: nil) (f a b) :: nil)
+
+        HNil HNil HNil c (Star Emp (Star Emp Emp)) (Star Emp (Star Emp Emp))).
+      Set Printing All.
+      
+
+      
+      
+      
+
+      Set Printing All
+canceler.
+      compute in H.
+      match goal with 
+        | [ |- @himp ?types ?funcs ?pcTyp ?stateTyp ?sfuncs _ _ _ _ _ _ ?cs ?L ?R ] =>
+          let R := fresh in
+            pose types ; pose funcs ;
+              pose pcTyp ; pose stateTyp ; pose sfuncs ;
+          pose (R := @CancelSep types funcs pcTyp stateTyp sfuncs cs nil L R)
+      end.
+      cbv beta iota zeta delta [CancelSep hash_left] in H.
+
+      match eval unfold H in H with
+        | ?X => idtac X
+        | match ?X as p return _ with 
+            | (_,_) => _
+          end _ => idtac X
+      end.
+
+      pose (sepCancel (SHeap_empty nil nil nil (nil ++ nil))
+              (liftSHeap nil nil nil
+                 (sheapSubstU nil nil (SHeap_empty  l0 l1 nil (nil ++ nil))))).
+      compute in p.
+
+      Set Printing All.
+
+      compute in H.
+      hnf in H.
+      simpl in H.
+          let K := eval hnf in R in 
+          match K with 
+            | @Prove _ _ _ _ _ _ _ _ _ _ ?L' ?R' ?S ?PF =>
+              simple eapply PF; unfold denote; simpl
+          end
+
+
+
+ canceler.
+*)
+    Abort.
+
+    Goal forall a b c x y, @ST.himp a b c (f _ _ (g y (x + x) 1)) (f _ _ 1).
+      intros. debug_reflect.
+    Abort.
+
+    Goal forall a b c, @ST.himp a b c 
+      (ST.star (f _ _ 2) (f _ _ 1))
+      (f _ _ 1).
+      intros. debug_reflect.
+    Abort.
+
+    Goal forall a b c, @ST.himp a b c 
+      (ST.ex (fun y : nat => ST.ex (fun x : bool => ST.star (f _ _ (g x 1 2)) (f _ _ 1) )))
+      (f _ _ 1).
+      intros. debug_reflect.
+    Abort.
+
+    Goal forall a b c, @ST.himp a b c 
+      (ST.ex (fun y : nat => f _ _ y))
+      (f _ _ 1).
+      intros. debug_reflect.
+    Abort.
+
+  End Tests.
